src/versions/standard/Int63/Int63Axioms_standard.v
@@ -17,6 +17,7 @@
 
 Require Import Bvector.
 Require Export BigNumPrelude.
+Require Import Int63Lib.
 Require Export Int63Native.
 Require Export Int63Op.
 
@@ -73,34 +74,34 @@ Axiom div_spec : forall x y, [|x / y|] = [|x|] / [|y|].
 Axiom mod_spec : forall x y, [|x \% y|] = [|x|] mod [|y|].
 
 (* Comparisons *)
-Axiom eqb_refl : forall x, (x == x)%int63 = true.
+Axiom eqb_refl : forall x, (x == x)%int = true.
 
-Axiom ltb_spec : forall x y, (x < y)%int63 = true <-> [|x|] < [|y|].
+Axiom ltb_spec : forall x y, (x < y)%int = true <-> [|x|] < [|y|].
 
-Axiom leb_spec : forall x y, (x <= y)%int63 = true <-> [|x|] <= [|y|].
+Axiom leb_spec : forall x y, (x <= y)%int = true <-> [|x|] <= [|y|].
 
 (** Iterators *)
 
 Axiom foldi_cont_gt : forall A B f from to cont,
-  (to < from)%int63 = true -> foldi_cont (A:=A) (B:=B) f from to cont = cont.
+  (to < from)%int = true -> foldi_cont (A:=A) (B:=B) f from to cont = cont.
 
 Axiom foldi_cont_eq : forall A B f from to cont,
   from = to -> foldi_cont (A:=A) (B:=B) f from to cont = f from cont.
 
 Axiom foldi_cont_lt : forall A B f from to cont,
-  (from < to)%int63 = true-> 
-  foldi_cont (A:=A) (B:=B) f from to cont = 
-  f from (fun a' => foldi_cont f (from+1) to cont a').
+  (from < to)%int = true->
+  foldi_cont (A:=A) (B:=B) f from to cont =
+  f from (fun a' => foldi_cont f (from + 1%int) to cont a').
 
 Axiom foldi_down_cont_lt : forall A B f from downto cont,
-  (from < downto)%int63 = true -> foldi_down_cont (A:=A) (B:=B) f from downto cont = cont.
+  (from < downto)%int = true -> foldi_down_cont (A:=A) (B:=B) f from downto cont = cont.
 
 Axiom foldi_down_cont_eq : forall A B f from downto cont,
   from = downto -> foldi_down_cont (A:=A) (B:=B) f from downto cont = f from cont.
 
 Axiom foldi_down_cont_gt : forall A B f from downto cont,
-  (downto < from)%int63 = true-> 
-  foldi_down_cont (A:=A) (B:=B) f from downto cont = 
+  (downto < from)%int = true->
+  foldi_down_cont (A:=A) (B:=B) f from downto cont =
   f from (fun a' => foldi_down_cont f (from-1) downto cont a').
 
 (** Print *)
@@ -117,11 +118,11 @@ Axiom head0_spec  : forall x,  0 < [|x|] ->
 Axiom tail0_spec  : forall x, 0 < [|x|] ->
          (exists y, 0 <= y /\ [|x|] = (2 * y + 1) * (2 ^ [|tail0 x|]))%Z.
 
-Axiom addc_def_spec : forall x y, (x +c y)%int63 = addc_def x y.
+Axiom addc_def_spec : forall x y, (x +c y)%int = addc_def x y.
 
 Axiom addcarryc_def_spec : forall x y, addcarryc x y = addcarryc_def x y.
 
-Axiom subc_def_spec : forall x y, (x -c y)%int63 = subc_def x y.
+Axiom subc_def_spec : forall x y, (x -c y)%int = subc_def x y.
 
 Axiom subcarryc_def_spec : forall x y, subcarryc x y = subcarryc_def x y.
 
