src/versions/standard/Int63/Int63Lib_standard.v
@@ -1,0 +1,454 @@
+(************************************************************************)
+(*  v      *   The Coq Proof Assistant  /  The Coq Development Team     *)
+(* <O___,, *   INRIA - CNRS - LIX - LRI - PPS - Copyright 1999-2014     *)
+(*   \VV/  **************************************************************)
+(*    //   *      This file is distributed under the terms of the       *)
+(*         *       GNU Lesser General Public License Version 2.1        *)
+(************************************************************************)
+(*            Benjamin Gregoire, Laurent Thery, INRIA, 2007             *)
+(************************************************************************)
+
+Require Import NaryFunctions.
+Require Import Wf_nat.
+Require Export ZArith.
+Require Export DoubleType.
+
+(** * 63-bit integers *)
+
+(** This file contains basic definitions of a 63-bit integer arithmetic.
+  It is based on the Int31 library, using its genericity. *)
+
+Definition size := 63%nat.
+
+(** Digits *)
+
+Inductive digits : Type := D0 | D1.
+
+(** The type of 63-bit integers *)
+
+(** The type [int63] has a unique constructor [I63] that expects
+   63 arguments of type [digits]. *)
+
+Definition digits63 t := Eval compute in nfun digits size t.
+
+Inductive int63 : Type := I63 : digits63 int63.
+
+Notation int := int63.
+
+(* spiwack: Registration of the type of integers, so that the matchs in
+   the functions below perform dynamic decompilation (otherwise some segfault
+   occur when they are applied to one non-closed term and one closed term). *)
+
+Delimit Scope int63_scope with int.
+Bind Scope int63_scope with int.
+Local Open Scope int63_scope.
+
+(** * Constants *)
+
+(** Zero is [I63 D0 ... D0] *)
+Definition On : int63 := Eval compute in napply_cst _ _ D0 size I63.
+Notation "0" := On : int63_scope.
+
+(** One is [I63 D0 ... D0 D1] *)
+Definition In : int63 := Eval compute in (napply_cst _ _ D0 (size-1) I63) D1.
+Notation "1" := In : int63_scope.
+
+(** The biggest integer is [I63 D1 ... D1], corresponding to [(2^size)-1] *)
+Definition Tn : int63 := Eval compute in napply_cst _ _ D1 size I63.
+
+(** Two is [I63 D0 ... D0 D1 D0] *)
+Definition Twon : int63 := Eval compute in (napply_cst _ _ D0 (size-2) I63) D1 D0.
+Notation "2" := Twon : int63_scope.
+
+(** * Bits manipulation *)
+
+
+(** [sneakr b x] shifts [x] to the right by one bit.
+   Rightmost digit is lost while leftmost digit becomes [b].
+   Pseudo-code is
+    [ match x with (I63 d0 ... dN) => I63 b d0 ... d(N-1) end ]
+*)
+
+Definition sneakr : digits -> int63 -> int63 := Eval compute in
+ fun b => int63_rect _ (napply_except_last _ _ (size-1) (I63 b)).
+
+(** [sneakl b x] shifts [x] to the left by one bit.
+   Leftmost digit is lost while rightmost digit becomes [b].
+   Pseudo-code is
+    [ match x with (I63 d0 ... dN) => I63 d1 ... dN b end ]
+*)
+
+Definition sneakl : digits -> int63 -> int63 := Eval compute in
+ fun b => int63_rect _ (fun _ => napply_then_last _ _ b (size-1) I63).
+
+
+(** [shiftl], [shiftr], [twice] and [twice_plus_one] are direct
+    consequences of [sneakl] and [sneakr]. *)
+
+Definition shiftl := sneakl D0.
+Definition shiftr := sneakr D0.
+Definition twice := sneakl D0.
+Definition twice_plus_one := sneakl D1.
+
+(** [firstl x] returns the leftmost digit of number [x].
+    Pseudo-code is [ match x with (I63 d0 ... dN) => d0 end ] *)
+
+Definition firstl : int63 -> digits := Eval compute in
+ int63_rect _ (fun d => napply_discard _ _ d (size-1)).
+
+(** [firstr x] returns the rightmost digit of number [x].
+    Pseudo-code is [ match x with (I63 d0 ... dN) => dN end ] *)
+
+Definition firstr : int63 -> digits := Eval compute in
+ int63_rect _ (napply_discard _ _ (fun d=>d) (size-1)).
+
+(** [iszero x] is true iff [x = I63 D0 ... D0]. Pseudo-code is
+    [ match x with (I63 D0 ... D0) => true | _ => false end ] *)
+
+Definition iszero : int63 -> bool := Eval compute in
+ let f d b := match d with D0 => b | D1 => false end
+ in int63_rect _ (nfold_bis _ _ f true size).
+
+(* NB: DO NOT transform the above match in a nicer (if then else).
+   It seems to work, but later "unfold iszero" takes forever. *)
+
+
+(** [base] is [2^63], obtained via iterations of [Z.double].
+   It can also be seen as the smallest b > 0 s.t. phi_inv b = 0
+   (see below) *)
+
+Definition base := Eval compute in
+ iter_nat size Z Z.double 1%Z.
+
+(** * Recursors *)
+
+Fixpoint recl_aux (n:nat)(A:Type)(case0:A)(caserec:digits->int63->A->A)
+ (i:int63) : A :=
+  match n with
+  | O => case0
+  | S next =>
+          if iszero i then
+             case0
+          else
+             let si := shiftl i in
+             caserec (firstl i) si (recl_aux next A case0 caserec si)
+  end.
+
+Fixpoint recr_aux (n:nat)(A:Type)(case0:A)(caserec:digits->int63->A->A)
+ (i:int63) : A :=
+  match n with
+  | O => case0
+  | S next =>
+          if iszero i then
+             case0
+          else
+             let si := shiftr i in
+             caserec (firstr i) si (recr_aux next A case0 caserec si)
+  end.
+
+Definition recl := recl_aux size.
+Definition recr := recr_aux size.
+
+(** * Conversions *)
+
+(** From int63 to Z, we simply iterates [Z.double] or [Z.succ_double]. *)
+
+Definition phi : int63 -> Z :=
+ recr Z (0%Z)
+  (fun b _ => match b with D0 => Z.double | D1 => Z.succ_double end).
+
+(** From positive to int63. An abstract definition could be :
+      [ phi_inv (2n) = 2*(phi_inv n) /\
+        phi_inv 2n+1 = 2*(phi_inv n) + 1 ] *)
+
+Fixpoint phi_inv_positive p :=
+  match p with
+    | xI q => twice_plus_one (phi_inv_positive q)
+    | xO q => twice (phi_inv_positive q)
+    | xH => In
+  end.
+
+(** The negative part : 2-complement  *)
+
+Fixpoint complement_negative p :=
+  match p with
+    | xI q => twice (complement_negative q)
+    | xO q => twice_plus_one (complement_negative q)
+    | xH => twice Tn
+  end.
+
+(** A simple incrementation function *)
+
+Definition incr : int63 -> int63 :=
+ recr int63 In
+   (fun b si rec => match b with
+     | D0 => sneakl D1 si
+     | D1 => sneakl D0 rec end).
+
+(** We can now define the conversion from Z to int63. *)
+
+Definition phi_inv : Z -> int63 := fun n =>
+ match n with
+ | Z0 => On
+ | Zpos p => phi_inv_positive p
+ | Zneg p => incr (complement_negative p)
+ end.
+
+(** [phi_inv2] is similar to [phi_inv] but returns a double word
+    [zn2z int63] *)
+
+Definition phi_inv2 n :=
+  match n with
+  | Z0 => W0
+  | _ => WW (phi_inv (n/base)%Z) (phi_inv n)
+  end.
+
+(** [phi2] is similar to [phi] but takes a double word (two args) *)
+
+Definition phi2 nh nl :=
+  ((phi nh)*base+(phi nl))%Z.
+
+(** * Addition *)
+
+(** Addition modulo [2^63] *)
+
+Definition add63 (n m : int63) := phi_inv ((phi n)+(phi m)).
+Notation "n + m" := (add63 n m) : int63_scope.
+
+(** Addition with carry (the result is thus exact) *)
+
+(* spiwack : when executed in non-compiled*)
+(* mode, (phi n)+(phi m) is computed twice*)
+(* it may be considered to optimize it *)
+
+Definition add63c (n m : int63) :=
+  let npm := n+m in
+  match (phi npm ?= (phi n)+(phi m))%Z with
+  | Eq => C0 npm
+  | _ => C1 npm
+  end.
+Notation "n '+c' m" := (add63c n m) (at level 50, no associativity) : int63_scope.
+
+(**  Addition plus one with carry (the result is thus exact) *)
+
+Definition add63carryc (n m : int63) :=
+  let npmpone_exact := ((phi n)+(phi m)+1)%Z in
+  let npmpone := phi_inv npmpone_exact in
+  match (phi npmpone ?= npmpone_exact)%Z with
+  | Eq => C0 npmpone
+  | _ => C1 npmpone
+  end.
+
+(** * Substraction *)
+
+(** Subtraction modulo [2^63] *)
+
+Definition sub63 (n m : int63) := phi_inv ((phi n)-(phi m)).
+Notation "n - m" := (sub63 n m) : int63_scope.
+
+(** Subtraction with carry (thus exact) *)
+
+Definition sub63c (n m : int63) :=
+  let nmm := n-m in
+  match (phi nmm ?= (phi n)-(phi m))%Z with
+  | Eq => C0 nmm
+  | _ => C1 nmm
+  end.
+Notation "n '-c' m" := (sub63c n m) (at level 50, no associativity) : int63_scope.
+
+(** subtraction minus one with carry (thus exact) *)
+
+Definition sub63carryc (n m : int63) :=
+  let nmmmone_exact := ((phi n)-(phi m)-1)%Z in
+  let nmmmone := phi_inv nmmmone_exact in
+  match (phi nmmmone ?= nmmmone_exact)%Z with
+  | Eq => C0 nmmmone
+  | _ => C1 nmmmone
+  end.
+
+(** Opposite *)
+
+Definition opp63 x := On - x.
+Notation "- x" := (opp63 x) : int63_scope.
+
+(** Multiplication *)
+
+(** multiplication modulo [2^63] *)
+
+Definition mul63 (n m : int63) := phi_inv ((phi n)*(phi m)).
+Notation "n * m" := (mul63 n m) : int63_scope.
+
+(** multiplication with double word result (thus exact) *)
+
+Definition mul63c (n m : int63) := phi_inv2 ((phi n)*(phi m)).
+Notation "n '*c' m" := (mul63c n m) (at level 40, no associativity) : int63_scope.
+
+
+(** * Division *)
+
+(** Division of a double size word modulo [2^63] *)
+
+Definition div6321 (nh nl m : int63) :=
+  let (q,r) := Z.div_eucl (phi2 nh nl) (phi m) in
+  (phi_inv q, phi_inv r).
+
+(** Division modulo [2^63] *)
+
+Definition div63 (n m : int63) :=
+  let (q,r) := Z.div_eucl (phi n) (phi m) in
+  (phi_inv q, phi_inv r).
+Notation "n / m" := (div63 n m) : int63_scope.
+
+
+(** * Unsigned comparison *)
+
+Definition compare63 (n m : int63) := ((phi n)?=(phi m))%Z.
+Notation "n ?= m" := (compare63 n m) (at level 70, no associativity) : int63_scope.
+
+Definition eqb63 (n m : int63) :=
+ match n ?= m with Eq => true | _ => false end.
+
+
+(** Computing the [i]-th iterate of a function:
+    [iter_int63 i A f = f^i] *)
+
+Definition iter_int63 i A f :=
+  recr (A->A) (fun x => x)
+   (fun b si rec => match b with
+      | D0 => fun x => rec (rec x)
+      | D1 => fun x => f (rec (rec x))
+    end)
+    i.
+
+(** Combining the [(63-p)] low bits of [i] above the [p] high bits of [j]:
+    [addmuldiv63 p i j = i*2^p+j/2^(63-p)]  (modulo [2^63]) *)
+
+Definition addmuldiv63 p i j :=
+ let (res, _ ) :=
+ iter_int63 p (int63*int63)
+  (fun ij => let (i,j) := ij in (sneakl (firstl j) i, shiftl j))
+  (i,j)
+ in
+ res.
+
+
+Fixpoint euler (guard:nat) (i j:int63) {struct guard} :=
+  match guard with
+    | O => In
+    | S p => match j ?= On with
+               | Eq => i
+               | _ => euler p j (let (_, r ) := i/j in r)
+             end
+  end.
+
+Definition gcd63 (i j:int63) := euler (2*size)%nat i j.
+
+(** Square root functions using newton iteration
+    we use a very naive upper-bound on the iteration
+    2^63 instead of the usual 63.
+**)
+
+
+
+Definition sqrt63_step (rec: int63 -> int63 -> int63) (i j: int63)  :=
+Eval lazy delta [Twon] in
+  let (quo,_) := i/j in
+  match quo ?= j with
+    Lt => rec i (fst ((j + quo)/Twon))
+  | _ =>  j
+  end.
+
+Fixpoint iter63_sqrt (n: nat) (rec: int63 -> int63 -> int63)
+          (i j: int63) {struct n} : int63 :=
+  sqrt63_step
+   (match n with
+      O =>  rec
+   | S n => (iter63_sqrt n (iter63_sqrt n rec))
+   end) i j.
+
+Definition sqrt63 i :=
+Eval lazy delta [On In Twon] in
+  match compare63 In i with
+    Gt => On
+  | Eq => In
+  | Lt => iter63_sqrt 63 (fun i j => j) i (fst (i/Twon))
+  end.
+
+Definition v30 := Eval compute in (addmuldiv63 (phi_inv (Z.of_nat size - 1)) In On).
+
+Definition sqrt632_step (rec: int63 -> int63 -> int63 -> int63)
+   (ih il j: int63)  :=
+Eval lazy delta [Twon v30] in
+  match ih ?= j with Eq => j | Gt => j | _ =>
+  let (quo,_) := div6321 ih il j in
+  match quo ?= j with
+    Lt => let m := match j +c quo with
+                    C0 m1 => fst (m1/Twon)
+                  | C1 m1 => fst (m1/Twon) + v30
+                  end in rec ih il m
+  | _ =>  j
+  end end.
+
+Fixpoint iter632_sqrt (n: nat)
+          (rec: int63  -> int63 -> int63 -> int63)
+          (ih il j: int63) {struct n} : int63 :=
+  sqrt632_step
+   (match n with
+      O =>  rec
+   | S n => (iter632_sqrt n (iter632_sqrt n rec))
+   end) ih il j.
+
+Definition sqrt632 ih il :=
+Eval lazy delta [On In] in
+  let s := iter632_sqrt 63 (fun ih il j => j) ih il Tn in
+           match s *c s with
+            W0 => (On, C0 On) (* impossible *)
+          | WW ih1 il1 =>
+             match il -c il1 with
+                C0 il2 =>
+                  match ih ?= ih1 with
+                    Gt => (s, C1 il2)
+                  | _  => (s, C0 il2)
+                  end
+              | C1 il2 =>
+                  match (ih - In) ?= ih1 with (* we could parametrize ih - 1 *)
+                    Gt => (s, C1 il2)
+                  | _  => (s, C0 il2)
+                  end
+              end
+          end.
+
+
+Fixpoint p2i n p : (N*int63)%type :=
+  match n with
+    | O => (Npos p, On)
+    | S n => match p with
+               | xO p => let (r,i) := p2i n p in (r, Twon*i)
+               | xI p => let (r,i) := p2i n p in (r, Twon*i+In)
+               | xH => (N0, In)
+             end
+  end.
+
+Definition positive_to_int63 (p:positive) := p2i size p.
+
+(** Constant 63 converted into type int63.
+    It is used as default answer for numbers of zeros
+    in [head0] and [tail0] *)
+
+Definition T63 : int63 := Eval compute in phi_inv (Z.of_nat size).
+
+Definition head063 (i:int63) :=
+  recl _ (fun _ => T63)
+   (fun b si rec n => match b with
+     | D0 => rec (add63 n In)
+     | D1 => n
+    end)
+   i On.
+
+Definition tail063 (i:int63) :=
+  recr _ (fun _ => T63)
+   (fun b si rec n => match b with
+     | D0 => rec (add63 n In)
+     | D1 => n
+    end)
+   i On.
