src/versions/standard/Int63/Int63_standard.v
@@ -14,6 +14,12 @@
 (*                                                                        *)
 (**************************************************************************)
 
+
+(** Naive software representation of Int63. To improve. Anyway, if you
+    want efficiency, rather use native-coq. **)
+
+Require Export Cyclic63.
+Require Export Ring63.
 Require Export Int63Native.
 Require Export Int63Op.
 Require Export Int63Axioms.
