src/configure.sh
@@ -5,6 +5,9 @@ set -e
 if [ $@ -a $@ = -standard ]; then
     cp versions/standard/Makefile Makefile
     cp versions/standard/Int63/Int63_standard.v versions/standard/Int63/Int63.v
+    cp versions/standard/Int63/Int63Lib_standard.v versions/standard/Int63/Int63Lib.v
+    cp versions/standard/Int63/Cyclic63_standard.v versions/standard/Int63/Cyclic63.v
+    cp versions/standard/Int63/Ring63_standard.v versions/standard/Int63/Ring63.v
     cp versions/standard/Int63/Int63Native_standard.v versions/standard/Int63/Int63Native.v
     cp versions/standard/Int63/Int63Op_standard.v versions/standard/Int63/Int63Op.v
     cp versions/standard/Int63/Int63Axioms_standard.v versions/standard/Int63/Int63Axioms.v
